Tables/Schema.lean
@@ -26,6 +26,17 @@ def getName (self : Schema) (i : Nat) (h : i < self.size := by get_elem_tactic) 
 def getDataType (self : Schema) (i : Nat) (h : i < self.size := by get_elem_tactic) : DataType :=
   self.specs[i].2
 
+def concat (self other : Schema) : Schema :=
+  { specs := self.specs ++ other.specs }
+
+instance : Append Schema where
+  append := concat
+
+theorem append_def (self other : Schema) : self ++ other = { specs := self.specs ++ other.specs } := (rfl)
+
+def selectNotByNames (self : Schema) (names : Array String) : Schema :=
+  { specs := self.specs.filter fun (name, _) => name ∉ names }
+
 end Schema
 
 end Tables
