Tables/Row/Lemmas.lean
@@ -21,6 +21,21 @@ theorem schema_getDataType_eq_getDataType (self : Row) (i : Nat) (h : i < self.s
     self.schema.getDataType i (self.schema_size_eq_size ▸ h) = self.getDataType i h := by
   grind [Row.schema, Row.getDataType, Schema.getDataType]
 
+@[simp, grind =]
+theorem concat_size (self other : Row) : (self.concat other).size = self.size + other.size := by
+  simp [Row.concat, Row.size]
+
+@[simp, grind =]
+theorem append_def (self other : Row) : self ++ other = { cells := self.cells ++ other.cells } := (rfl)
+
+@[simp, grind =]
+theorem append_schema (self other : Row) : (self ++ other).schema = self.schema ++ other.schema := by
+  simp [Row.schema, Schema.append_def]
+
+@[simp, grind =]
+theorem selectNotByNames_schema (self : Row) (names : Array String) : (self.selectNotByNames names).schema = self.schema.selectNotByNames names := by
+  simp only [schema, selectNotByNames, decide_not, Schema.selectNotByNames, Array.filter_map, Function.comp_def]
+
 end Tables.Row
 
 end
