Tables/Table/Raw/Join.lean
@@ -1,0 +1,78 @@
+module
+
+public import Tables.Table.Raw.Basic
+import all Tables.Table.Raw.Basic
+import Std.Data.HashMap
+import Std.Data.HashSet
+
+open Std (HashMap HashSet)
+
+public section
+
+namespace Tables.Table.Raw
+
+def distinct (self : Raw) (h : ∀ column ∈ self.columns, column.size = self.nrows) : Raw :=
+  let schema := self.schema
+
+  -- TODO: Rewrite other loops using similar Nat.fold pattern.
+  let rows : Array { row : Row // row.schema = schema } := Prod.snd <| Nat.fold (init := (∅, #[])) self.nrows fun i isLt (seen, rows) =>
+    let row := self.getRow i isLt h
+    if row ∈ seen then
+      (seen, rows)
+    else
+      have h' : row.schema = schema := by
+        simp [row, getRow_schema, schema]
+      (HashSet.insert seen row, rows.push ⟨row, h'⟩)
+
+  ofRows schema rows.unattach (by grind [Array.mem_unattach])
+
+def crossJoin (self other : Raw)
+    (h₁ : ∀ column ∈ self.columns, column.size = self.nrows) (h₂ : ∀ column ∈ other.columns, column.size = other.nrows) : Raw :=
+  let schema := self.schema ++ other.schema
+  let rows := Array.flatten <| Array.ofFn fun (i : Fin self.nrows) =>
+    Array.ofFn fun (j : Fin other.nrows) =>
+      self.getRow i i.isLt h₁ ++ other.getRow j j.isLt h₂
+  have h (row : Row) (mem : row ∈ rows) : row.schema = schema := by
+    rw [Array.mem_flatten] at mem
+    obtain ⟨xs, h, mem⟩ := mem
+    rw [Array.mem_ofFn] at h
+    obtain ⟨i, eq⟩ := h
+    rw [←eq, Array.mem_ofFn] at mem
+    obtain ⟨j, eq⟩ := mem
+    grind only [= Row.append_schema, = getRow_schema]
+  ofRows schema rows h
+
+def leftJoin (self other : Raw) (keys : Array String)
+    (h₁ : ∀ column ∈ self.columns, column.size = self.nrows) (h₂ : ∀ column ∈ other.columns, column.size = other.nrows) : Raw :=
+  let schema := self.schema ++ other.schema.selectNotByNames keys
+
+  let otherRowsMap : HashMap Row (Array (Fin other.nrows)) := Nat.fold (init := ∅) other.nrows fun i isLt m =>
+    let row := other.getRow i isLt h₂
+    let keyRow := row.selectByNames keys
+    m.alter keyRow fun
+      | some xs => some (xs.push ⟨i, isLt⟩)
+      | none => some #[⟨i, isLt⟩]
+  let rows : Array Row := Array.flatten <| (Array.finRange self.nrows).map fun i =>
+    let row := self.getRow i.val i.isLt h₁
+    let keyRow := row.selectByNames keys
+    match otherRowsMap.get? keyRow with
+    | some ns =>
+      let newRows := ns.map fun j => row ++ (other.getRow j.val j.isLt h₂).selectNotByNames keys
+      newRows
+    | none => #[]
+
+  have h (row : Row) (mem : row ∈ rows) : row.schema = schema := by
+    simp only [HashMap.get?_eq_getElem?, Array.mem_flatten, Array.mem_map, rows] at mem
+    obtain ⟨xs, ⟨i, mem, eq⟩, mem'⟩ := mem
+    split at eq
+    next ns eq' =>
+      subst xs
+      simp only [Array.mem_map] at mem'
+      obtain ⟨n, mem'', eq''⟩ := mem'
+      simp only [←eq'', Row.append_schema, getRow_schema, Row.selectNotByNames_schema, schema]
+    next => grind
+  ofRows schema rows h
+
+end Tables.Table.Raw
+
+end
